bin/gen/ExtractRomanWheel.v
@@ -18,4 +18,6 @@ Require Import TBGen.TB.TB.
 
 Set Warnings "-extraction-default-directory".
 
+Extract Constant PeanoNat.Nat.modulo => "fun x y -> x mod y".
+
 Extraction "TBGen.ml" RW_TB.
